wand_demo/wand_frame.v
@@ -1,0 +1,19 @@
+Require Import msl.seplog.
+Require Import msl.log_normalize.
+Local Open Scope logic.
+
+Lemma wf_intro {A} {ND: NatDed A} {SL: SepLog A}: forall (P Q: A),
+  Q |-- P -* P * Q.
+Proof.
+  intros.
+  apply wand_sepcon_adjoint.
+  rewrite sepcon_comm; auto.
+Qed.
+
+Lemma wf_elim {A} {ND: NatDed A} {SL: SepLog A}: forall (P Q: A),
+  P * (P -* Q) |-- Q.
+Proof.
+  intros.
+  rewrite sepcon_comm.
+  apply wand_sepcon_adjoint; auto.
+Qed.
