Makefile
@@ -232,8 +232,9 @@ FLOYD_FILES= \
 #real_forward.v
 
 WAND_DEMO_FILES= \
-   list.v list_lemmas.v verif_list.v \
-   bst.v
+  wand_frame.v \
+  list.v list_lemmas.v verif_list.v \
+  bst.v
 
 # CONCPROGS must be kept separate (see util/PACKAGE), and
 # each line that contains the word CONCPROGS must be deletable independently
